timing/riscv/NEORV32.v
@@ -1,6 +1,8 @@
-Require Import CPUTimingBehavior.
-Require Import NArith.
-Require Import Picinae_core.
+Require Import CPUTimingBehavior ProgramInformation.
+Require Import NArith ZArith.
+Require Import Picinae_riscv.
+Import RISCVNotations.
+Open Scope r5_scope.
 Open Scope N.
 
 (* https://stnolting.github.io/neorv32/#_processor_top_entity_generics *)
@@ -13,12 +15,38 @@ Module Type NEORV32Config.
     Parameter CPU_FAST_MUL_EN : bool.
     (* Implement the instruction cache *)
     Parameter ICACHE_EN : bool.
+    (* Number of instruction cache lines *)
+    Parameter ICACHE_NUM_BLOCKS : N.
     (* Implement the data cache *)
     Parameter DCACHE_EN : bool.
+    (* Number of data cache lines *)
+    Parameter DCACHE_NUM_BLOCKS : N.
+    (* Size of a cache line *)
+    Parameter CACHE_BLOCK_SIZE : N.
 End NEORV32Config.
 
+Record cache_line : Type := {
+    tag : N;
+    data : memory;
+    initialized : bool
+}.
+
+Inductive cache_type : Type :=
+    | Data | Instruction.
+
+Record cache : Type := {
+    iline : N -> cache_line;
+    dline : N -> cache_line;
+}.
+
+Fixpoint range (n : N) : list N.
+    destruct n as [| n' IHn'] using (N.peano_rect).
+        exact nil.
+    exact (List.cons n' IHn').
+Defined.
+
 (* https://stnolting.github.io/neorv32/#_instruction_sets_and_extensions *)
-Module NEORV32 (cfg : NEORV32Config) <: CPUTimingBehavior.
+Module NEORV32 (cfg : NEORV32Config) (prog : ProgramInformation) <: CPUTimingBehavior.
     (* Latency Definitions *)
     Definition T_shift_latency (offset : N) : N :=
         if cfg.CPU_FAST_SHIFT_EN then
@@ -32,8 +60,127 @@ Module NEORV32 (cfg : NEORV32Config) <: CPUTimingBehavior.
         else
             32.
 
-    Parameter T_data_latency : N.
-    Parameter T_inst_latency : N.
+    Definition cache : Type := cache.
+
+    Definition clear_cache : cache :=
+        {|iline := fun _ => {|tag := 0; data := 0; initialized := false|};
+          dline := fun _ => {|tag := 0; data := 0; initialized := false|}|}.
+
+    Definition cache_read (s : store) (c : cache) 
+            (address : addr) (ct : cache_type) : cache :=
+        let '(CACHE, CACHE_LINES) := (
+             match ct with 
+             | Instruction => (c.(iline), cfg.ICACHE_NUM_BLOCKS)
+             | Data => (c.(dline), cfg.DCACHE_NUM_BLOCKS)
+             end) in
+        let offset := address mod cfg.CACHE_BLOCK_SIZE in
+        let index := (address / cfg.CACHE_BLOCK_SIZE) mod CACHE_LINES in
+        let tag' := address / (cfg.CACHE_BLOCK_SIZE * CACHE_LINES) in
+        
+        let line := CACHE index in
+
+        if andb (line.(initialized)) (line.(tag) =? tag') then (
+            c
+        ) else (
+            let base_addr := address - offset in
+            let line' := {| data := List.fold_left (fun data i =>
+                data [Ⓑ i := (s V_MEM32) Ⓑ[base_addr + i]]
+            ) (range cfg.CACHE_BLOCK_SIZE) (line.(data));
+               tag := tag';
+               initialized := true |} in
+            match ct with
+            | Data =>
+                {|dline := update c.(dline) index line'; iline := c.(iline)|}
+            | Instruction =>
+                {|dline := c.(dline); iline := update c.(iline) index line'|}
+            end
+        ).
+
+    Definition cache_write (c : cache) 
+            (address : addr) (value : N) (ct : cache_type) : cache :=
+        let '(CACHE, CACHE_LINES) := (
+             match ct with 
+             | Instruction => (c.(iline), cfg.ICACHE_NUM_BLOCKS)
+             | Data => (c.(dline), cfg.DCACHE_NUM_BLOCKS)
+             end) in
+        let offset := address mod cfg.CACHE_BLOCK_SIZE in
+        let index := (address / cfg.CACHE_BLOCK_SIZE) mod CACHE_LINES in
+        let tag' := address / (cfg.CACHE_BLOCK_SIZE * CACHE_LINES) in
+        
+        let line := CACHE index in
+
+        if line.(tag) =? tag' then (
+            let line' :=
+                {|data := line.(data) [Ⓓ offset := value];
+                  tag := tag';
+                  initialized := true|} in
+            match ct with
+            | Data =>
+                {|dline := update c.(dline) index line'; iline := c.(iline)|}
+            | Instruction =>
+                {|dline := c.(dline); iline := update c.(iline) index line'|}
+            end
+        ) else (
+            c
+        ).
+
+    Definition cached (c : cache) (address : addr) (ct : cache_type) : bool :=
+         let '(CACHE, CACHE_LINES) := (
+             match ct with 
+             | Instruction => (c.(iline), cfg.ICACHE_NUM_BLOCKS)
+             | Data => (c.(dline), cfg.DCACHE_NUM_BLOCKS)
+             end) in
+        let index := (address / cfg.CACHE_BLOCK_SIZE) mod CACHE_LINES in
+        let tag' := address / (cfg.CACHE_BLOCK_SIZE * CACHE_LINES) in
+
+        (CACHE index).(tag) =? tag'.
+
+    Definition cache_step (s : store) (c : cache) (a : addr) : cache :=
+        let load a o := cache_read s c 
+            (add_signed_offset' (reg s a) o) Data in
+        let write a o v := cache_write c 
+            (add_signed_offset (reg s a) o)
+            (reg s v) Data in
+        let jump a' := cache_read s c (add_signed_offset a a') Instruction in
+        match rv_decode (prog.binary a) with
+        | R5_Lb _ rs imm => load rs imm
+        | R5_Lh _ rs imm => load rs imm
+        | R5_Lw _ rs imm => load rs imm
+        | R5_Lbu _ rs imm => load rs imm
+        | R5_Lhu _ rs imm => load rs imm
+        | R5_Sb rs2 rs1 imm => write rs1 imm rs2
+        | R5_Sh rs2 rs1 imm => write rs1 imm rs2
+        | R5_Sw rs2 rs1 imm => write rs1 imm rs2
+        | R5_Fence _ _ => clear_cache
+        | R5_Fence_i => clear_cache
+        | R5_Beq _ _ a => jump a
+        | R5_Bne _ _ a => jump a
+        | R5_Blt _ _ a => jump a
+        | R5_Bge _ _ a => jump a
+        | R5_Bltu _ _ a => jump a
+        | R5_Bgeu _ _ a => jump a
+        | R5_Jal _ a => jump a
+        | R5_Jalr r1 _ a =>
+            cache_read s c (resolve_jalr_addr a r1) Instruction
+        | _ => c
+        end.
+
+    Parameter T_data_latency_raw : N.
+    Parameter T_inst_latency_raw : N.
+
+    Definition T_data_latency (c : cache) (a : addr) : N :=
+        if cfg.DCACHE_EN then (
+            if cached c a Data then 1 else T_inst_latency_raw
+        ) else (
+            T_inst_latency_raw
+        ).
+
+    Definition T_inst_latency (c : cache) (a : addr) : N :=
+        if cfg.ICACHE_EN then (
+            if cached c a Instruction then 1 else T_inst_latency_raw
+        ) else (
+            T_inst_latency_raw
+        ).
 
     (* ==== I ISA Extension ==== *)
     (* ALU *)
@@ -67,38 +214,39 @@ Module NEORV32 (cfg : NEORV32Config) <: CPUTimingBehavior.
         3 + T_shift_latency offset.
     (* Branches *)
     (* taken *)
-    Definition ttbeq := 5 + T_inst_latency.
-    Definition ttbne := 5 + T_inst_latency.
-    Definition ttblt := 5 + T_inst_latency.
-    Definition ttbge := 5 + T_inst_latency.
-    Definition ttbltu := 5 + T_inst_latency.
-    Definition ttbgeu := 5 + T_inst_latency.
+    Definition ttbeq c a := 5 + T_inst_latency c a.
+    Definition ttbne c a := 5 + T_inst_latency c a.
+    Definition ttblt c a := 5 + T_inst_latency c a.
+    Definition ttbge c a := 5 + T_inst_latency c a.
+    Definition ttbltu c a := 5 + T_inst_latency c a.
+    Definition ttbgeu c a := 5 + T_inst_latency c a.
     (* not taken *)
-    Definition tfbeq := 3.
-    Definition tfbne := 3.
-    Definition tfblt := 3.
-    Definition tfbge := 3.
-    Definition tfbltu := 3.
-    Definition tfbgeu := 3.
+    Definition tfbeq (_ : cache) (_ : addr) := 3.
+    Definition tfbne (_ : cache) (_ : addr)  := 3.
+    Definition tfblt (_ : cache) (_ : addr)  := 3.
+    Definition tfbge (_ : cache) (_ : addr)  := 3.
+    Definition tfbltu (_ : cache) (_ : addr)  := 3.
+    Definition tfbgeu (_ : cache) (_ : addr)  := 3.
     (* Jump/call *)
-    Definition tjal := 5 + T_inst_latency.
-    Definition tjalr := 5 + T_inst_latency.
+    Definition tjal c a := 5 + T_inst_latency c a.
+    Definition tjalr c a := 5 + T_inst_latency c a.
     (* Load/store *)
-    Definition tlb := 4 + T_data_latency.
-    Definition tlh := 4 + T_data_latency.
-    Definition tlw := 4 + T_data_latency.
-    Definition tlbu := 4 + T_data_latency.
-    Definition tlhu := 4 + T_data_latency.
-    Definition tsb := 4 + T_data_latency.
-    Definition tsh := 4 + T_data_latency.
-    Definition tsw := 4 + T_data_latency.
+    Definition tlb c a := 4 + T_data_latency c a.
+    Definition tlh c a := 4 + T_data_latency c a.
+    Definition tlw c a := 4 + T_data_latency c a.
+    Definition tlbu c a := 4 + T_data_latency c a.
+    Definition tlhu c a := 4 + T_data_latency c a.
+    Definition tsb c a := 4 + T_data_latency c a.
+    Definition tsh c a := 4 + T_data_latency c a.
+    Definition tsw c a := 4 + T_data_latency c a.
     (* Data fence *)
-    Definition tfence := 6 + T_data_latency.
+    Definition tfence c := 6 + T_data_latency c 0.
+    Definition tfencei c := 6 + T_data_latency c 0.
     (* System *)
-    Definition tecall := 7 + T_inst_latency.
-    Definition tebreak := 7 + T_inst_latency.
-    Definition tmret := 7 + T_inst_latency.
-    Definition twfi := 7 + T_inst_latency.
+    Definition tecall c := 7 + T_inst_latency c 0.
+    Definition tebreak c := 7 + T_inst_latency c 0.
+    Definition tmret c := 7 + T_inst_latency c 0.
+    Definition twfi := 3.
 
     (* ==== M ISA Extension ==== *)
     (* Multiplication *)
@@ -158,6 +306,9 @@ Module NEORV32BaseConfig <: NEORV32Config.
     Definition CPU_FAST_MUL_EN : bool := false.
     Definition ICACHE_EN : bool := false.
     Definition DCACHE_EN : bool := false.
+    Definition ICACHE_NUM_BLOCKS : N := 4.
+    Definition DCACHE_NUM_BLOCKS : N := 4.
+    Definition CACHE_BLOCK_SIZE : N := 64.
 End NEORV32BaseConfig.
 
 Module NEORV32Base := NEORV32 NEORV32BaseConfig.
