timing/riscv/CPUTimingBehavior.v
@@ -1,27 +1,49 @@
-Require Import NArith.
+From Picinae Require Import Picinae_riscv.
+Require Import NArith ZArith.
+
+Definition resolve_jalr_addr (offset : Z) (a : addr) : addr :=
+        N.clearbit (ofZ 32 (Z.add offset (toZ 32 a))) 0.
+
+Definition add_signed_offset (a : N) (o : Z) : N :=
+    ofZ 32 (Z.add (toZ 32 a) o).
+
+Definition add_signed_offset' (a o : N) : N :=
+    ofZ 32 (Z.add (toZ 32 a) (toZ 32 o)).
+
+Definition reg s n := match n with 0 => 0 | _ => s (rv_varid n) end.
 
 Module Type CPUTimingBehavior.
+    Parameter cache : Type.
+    Parameter cache_step : store -> cache -> addr -> cache.
+
     (* === Instruction Timings === *)
     Parameter
         (* ==== I ISA Extension ==== *)
         (* ALU *)
             tadd taddi tslt tslti tsltu tsltiu
             txor txori tor tori tand tandi tsub tlui
-            tauipc
+            tauipc : N.
+    Parameter
         (* Branches *)
             (* taken *)
                 ttbeq ttbne ttblt ttbge ttbltu ttbgeu
             (* not taken *)
                 tfbeq tfbne tfblt tfbge tfbltu tfbgeu
         (* Jump/call *)
-            tjal tjalr
+            tjal tjalr : cache -> addr -> N.
+    Parameter
         (* Load/store *)
             tlb tlh tlw tlbu tlhu tsb tsh tsw
+            : cache -> N -> N.
+    Parameter
         (* Data fence *)
-            tfence
+            tfence tfencei : cache -> N.
+    Parameter
         (* System *)
-            tecall tebreak tmret twfi
-
+            tecall tebreak tmret : cache -> N. 
+    Parameter 
+        (* System *) 
+            twfi
         (* ==== M ISA Extension ==== *)
         (* Multiplication *)
             tmul tmulh tmulhsu tmulhu
