timing/riscv/ProgramInformation.v
@@ -1,0 +1,9 @@
+Require Import Picinae_riscv.
+Require Import NArith.
+
+Module Type ProgramInformation.
+    Parameter entry_addr : addr.
+    Parameter exits : trace -> bool.
+    (* Binary representation of the program to be decoded *)
+    Parameter binary : addr -> N.
+End ProgramInformation.
